SecureMessaging/CKA/FromKEM/Security/PrefixSim.lean
@@ -1,6 +1,7 @@
 /-
 Copyright (c) 2026 Beneficial AI Foundation. All rights reserved.
 Released under Apache 2.0 license as described in the file LICENSE.
+Authors: Beneficial AI Foundation
 -/
 
 import SecureMessaging.CKA.FromKEM.Security.HiddenStateSim
@@ -100,7 +101,7 @@ private lemma securityImpl_challA_preAToB_real_run
       (preAToBHonestState σ pkStar skStar) = _
   simp [CKAScheme.oracleChallA, scheme, send, preAToBHonestState,
     postAToBHonestState, CKAScheme.isChallengeEpoch, CKAScheme.GameState.tP,
-    hvalid, hparty, ht, stateT_run,
+    hvalid, hparty, ht, stateTrun,
     map_eq_bind_pure_comp]
   rfl
 
@@ -137,7 +138,7 @@ private lemma securityImpl_challA_preAToB_random_run
       (preAToBHonestState σ pkStar skStar) = _
   simp [CKAScheme.oracleChallA, scheme, send, preAToBHonestState,
     postAToBHonestState, CKAScheme.isChallengeEpoch, CKAScheme.GameState.tP,
-    hvalid, hparty, ht, stateT_run,
+    hvalid, hparty, ht, stateTrun,
     map_eq_bind_pure_comp]
   rfl
 
@@ -173,7 +174,7 @@ private lemma securityImpl_challB_preBToA_real_run
       (preBToAHonestState σ pkStar skStar) = _
   simp [CKAScheme.oracleChallB, scheme, send, preBToAHonestState,
     postBToAHonestState, CKAScheme.isChallengeEpoch, CKAScheme.GameState.tP,
-    hvalid, hparty, ht, stateT_run,
+    hvalid, hparty, ht, stateTrun,
     map_eq_bind_pure_comp]
   rfl
 
@@ -210,7 +211,7 @@ private lemma securityImpl_challB_preBToA_random_run
       (preBToAHonestState σ pkStar skStar) = _
   simp [CKAScheme.oracleChallB, scheme, send, preBToAHonestState,
     postBToAHonestState, CKAScheme.isChallengeEpoch, CKAScheme.GameState.tP,
-    hvalid, hparty, ht, stateT_run,
+    hvalid, hparty, ht, stateTrun,
     map_eq_bind_pure_comp]
   rfl
 
